code/ecdsa/Hacl.Impl.ECDSA.MontgomeryMultiplication.fsti
@@ -14,35 +14,17 @@ open Spec.ECC.Curves
 open Hacl.Spec.ECDSA.Definition
 open Spec.ECDSA
 open Hacl.Impl.P256.LowLevel 
-  
+open Hacl.Impl.EC.Setup
 
 open FStar.Mul
 
 noextract
-let prime = prime_p256_order
-
-inline_for_extraction
-let prime256order_buffer: x: glbuffer uint64 (size 4)  
-  {witnessed #uint64 #(size 4) x 
-  (Lib.Sequence.of_list p256_order_prime_list) /\ recallable x /\ 
-  felem_seq_as_nat (Lib.Sequence.of_list (p256_order_prime_list)) == prime_p256_order} = 
-  createL_global p256_order_prime_list
-
-
-inline_for_extraction
-let order_inverse_buffer: x: glbuffer uint8 32ul {witnessed x (prime_order_inverse_seq #P256) /\ recallable x} = 
-  createL_global (prime_order_inverse_list #P256)
-
-
-inline_for_extraction
-let order_buffer: x: glbuffer uint8 32ul {witnessed x (prime_order_seq #P256) /\ recallable x} = 
-  createL_global (prime_order_list #P256)
-
+let prime = (getOrder #P256)
 
 val reduction_prime_2prime_with_carry: #c: curve -> x: widefelem c -> result: felem c ->
   Stack unit 
-    (requires fun h -> live h x /\ live h result /\  eq_or_disjoint x result /\ wide_as_nat c h x < 2 * prime_p256_order)
-    (ensures fun h0 _ h1 -> modifies (loc result) h0 h1 /\ as_nat c h1 result = wide_as_nat c h0 x % prime_p256_order)  
+    (requires fun h -> live h x /\ live h result /\  eq_or_disjoint x result /\ wide_as_nat c h x < 2 * (getOrder #P256))
+    (ensures fun h0 _ h1 -> modifies (loc result) h0 h1 /\ as_nat c h1 result = wide_as_nat c h0 x % (getOrder #P256))  
 
 
 inline_for_extraction noextract
@@ -50,16 +32,16 @@ val reduction_prime_2prime_with_carry2: #c: curve ->  carry: uint64 ->  x: felem
   -> result: felem c ->
   Stack unit 
     (requires fun h -> live h x /\ live h result /\ eq_or_disjoint x result /\ 
-      uint_v carry * pow2 256 + as_nat c h x < 2 * prime_p256_order )
+      uint_v carry * pow2 256 + as_nat c h x < 2 * (getOrder #P256) )
     (ensures fun h0 _ h1 -> modifies (loc result) h0 h1 /\ 
-      as_nat c h1 result = (uint_v carry * pow2 256 + as_nat c h0 x) % prime_p256_order)  
+      as_nat c h1 result = (uint_v carry * pow2 256 + as_nat c h0 x) % (getOrder #P256))  
 
 
 val reduction_prime_2prime_order: #c: curve -> x: felem c 
   -> result: felem c -> 
   Stack unit 
     (requires fun h -> live h x /\ live h result /\ eq_or_disjoint x result)
-    (ensures fun h0 _ h1 -> modifies (loc result) h0 h1 /\  as_nat c h1 result == as_nat c h0 x % prime_p256_order)  
+    (ensures fun h0 _ h1 -> modifies (loc result) h0 h1 /\  as_nat c h1 result == as_nat c h0 x % (getOrder #P256))  
 
 
 noextract
@@ -69,10 +51,10 @@ noextract
 val toDomain_: a: nat -> Tot nat
 
 val lemmaFromDomain: a: nat ->  Lemma (
-  (a * modp_inv2_prime (pow2 256) prime_p256_order) % prime_p256_order == fromDomain_ a)
+  (a * modp_inv2_prime (pow2 256) (getOrder #P256)) % (getOrder #P256) == fromDomain_ a)
 
 val lemmaToDomain: a: nat ->  Lemma (
-  (a * pow2 256) % prime_p256_order == toDomain_ a)
+  (a * pow2 256) % (getOrder #P256) == toDomain_ a)
 
 
 val lemmaFromDomainToDomain: a: nat { a < prime} -> Lemma (toDomain_ (fromDomain_ a) == a)
@@ -84,20 +66,20 @@ val montgomery_multiplication_ecdsa_module: #c: curve -> a: felem c -> b: felem 
   ->result: felem c -> 
   Stack unit 
     (requires fun h -> live h a /\ live h b /\ live h result /\
-      as_nat c h a < prime_p256_order /\ as_nat c h b < prime_p256_order)
+      as_nat c h a < (getOrder #P256) /\ as_nat c h b < (getOrder #P256))
     (ensures fun h0 _ h1 -> 
       modifies (loc result) h0 h1 /\ 
-      as_nat c h1 result = (as_nat c h0 a * as_nat c h0 b * modp_inv2_prime (pow2 256) prime_p256_order) % prime_p256_order /\ 
-      as_nat c h1 result = toDomain_ (fromDomain_ (as_nat c h0 a) * fromDomain_ (as_nat c h0 b) % prime_p256_order))
+      as_nat c h1 result = (as_nat c h0 a * as_nat c h0 b * modp_inv2_prime (pow2 256) (getOrder #P256)) % (getOrder #P256) /\ 
+      as_nat c h1 result = toDomain_ (fromDomain_ (as_nat c h0 a) * fromDomain_ (as_nat c h0 b) % (getOrder #P256)))
 
 
 val felem_add: #c: curve -> arg1: felem c -> arg2: felem c -> out: felem c -> Stack unit 
   (requires (fun h0 ->  
     live h0 arg1 /\ live h0 arg2 /\ live h0 out /\ 
     eq_or_disjoint arg1 out /\ eq_or_disjoint arg2 out /\
-    as_nat c h0 arg1 < prime_p256_order /\ as_nat c h0 arg2 < prime_p256_order
+    as_nat c h0 arg1 < (getOrder #P256) /\ as_nat c h0 arg2 < (getOrder #P256)
    )
   )
-  (ensures (fun h0 _ h1 -> modifies (loc out) h0 h1 /\ as_nat c h1 out == (as_nat c h0 arg1 + as_nat c h0 arg2) % prime_p256_order))
+  (ensures (fun h0 _ h1 -> modifies (loc out) h0 h1 /\ as_nat c h1 out == (as_nat c h0 arg1 + as_nat c h0 arg2) % (getOrder #P256)))
 
-val lemma_felem_add: a: nat -> b: nat -> Lemma ((fromDomain_ a + fromDomain_ b) % prime_p256_order = fromDomain_ (a + b))
+val lemma_felem_add: a: nat -> b: nat -> Lemma ((fromDomain_ a + fromDomain_ b) % (getOrder #P256) = fromDomain_ (a + b))
